base cases (bool, nat, abs; not var yet) for subset proof

coq/two/LambdaTwo.v
@@ -1,6 +1,7 @@
 Require Import Recdef.
 Require Export LambdaTwoSyntax.
 Require Export IndistinguishabilityTwo.
+Require Import LibTactics.
 
 Definition pair_add (a : nat * nat) : nat :=
   match a with
@@ -62,11 +63,11 @@ Definition eval_kl : nat * nat -> two -> (value -> value -> Prop) ->
                   a = Atom (VClos e t') pc
                 | TApp t1 t2 =>
                   if Compare_dec.zerop (fst kl) then False else
-                    let eval := eval_kl (fst kl - 1, snd kl) _ L P in
+                    let eval := eval_kl (fst kl - 1, snd kl) _ in
                     exists e1' t1' l1 a2 a3,
-                      eval pc e t1 (Atom (VClos e1' t1') l1) /\
-                      eval pc e t2 a2 /\
-                      eval l1 (a2 :: e1') t1' a3 /\
+                      eval L P pc e t1 (Atom (VClos e1' t1') l1) /\
+                      eval L P pc e t2 a2 /\
+                      eval L P l1 (a2 :: e1') t1' a3 /\
                       a = a3
                 | TDecl t1 t2 =>
                   if Compare_dec.zerop (fst kl) then False else
@@ -76,10 +77,10 @@ Definition eval_kl : nat * nat -> two -> (value -> value -> Prop) ->
                       eval pc e t2 a2 /\
                       eval l1 (a2 :: e1') t1' (Atom v3 l3) /\
                       if bottomp l3 then a = Atom v3 Bottom2 else
-                        let eval := eval_kl (snd kl, fst kl - 1) _ L P in
+                        let eval := eval_kl (snd kl, fst kl - 1) _ in
                         (forall a2' e2' v3',
                            env_LPequiv L P (a2 :: e1') (a2' :: e2') ->
-                           eval l1 (a2' :: e2') t1' (Atom v3' Top2) ->
+                           eval L P l1 (a2' :: e2') t1' (Atom v3' Top2) ->
                            value_LPequiv L P v3 v3') /\
                         a = Atom v3 Bottom2
               end));
@@ -87,6 +88,78 @@ Definition eval_kl : nat * nat -> two -> (value -> value -> Prop) ->
       (destruct kl; auto); rewrite H; simpl; clear H;
   inversion _H; unfold pair_lt; auto.
 Defined.
+
+Lemma eval_kl_bool :
+  forall k l L P pc e b,
+    eval_kl (k, l) L P pc e (TBool b) (Atom (VBool b) pc).
+Proof.
+  intros. destruct k; destruct l; reflexivity.
+Qed.
+
+Lemma eval_kl_bool_inv :
+  forall k l L P pc e b a,
+    eval_kl (k, l) L P pc e (TBool b) a ->
+    a = Atom (VBool b) pc.
+Proof.
+  introv Heval.
+  destruct a as [v1 l1]; destruct v1 as [b1 | n1 | e1 t1];
+  destruct k; destruct l; inversion Heval; auto.
+Qed.
+
+Lemma eval_kl_nat :
+  forall k l L P pc e n,
+    eval_kl (k, l) L P pc e (TNat n) (Atom (VNat n) pc).
+Proof.
+  intros. destruct k; destruct l; reflexivity.
+Qed.
+
+Lemma eval_kl_nat_inv :
+  forall k l L P pc e n a,
+    eval_kl (k, l) L P pc e (TNat n) a ->
+    a = Atom (VNat n) pc.
+Proof.
+  introv Heval.
+  destruct a as [v1 l1]; destruct v1 as [b1 | n1 | e1 t1];
+  destruct k; destruct l; inversion Heval; auto.
+Qed.
+
+Lemma eval_kl_var :
+  forall k l L P pc e n v' l',
+    atIndex e n = Some (Atom v' l') ->
+    eval_kl (k, l) L P pc e (TVar n) (Atom v' (l' ⊔ pc)).
+Proof.
+  (* TODO *)
+  admit.
+Qed.
+
+Lemma eval_kl_var_inv :
+  forall k l L P pc e n a,
+    eval_kl (k, l) L P pc e (TVar n) a ->
+    exists v' l',
+      atIndex e n = Some (Atom v' l') /\
+      a = Atom v' (l' ⊔ pc).
+Proof.
+  introv Heval.
+  destruct a as [v1 l1]; destruct v1 as [b1 | n1 | e1 t1];
+  destruct k; destruct l; inversion Heval; auto.
+Qed.
+      
+Lemma eval_kl_abs :
+  forall k l L P pc e t',
+    eval_kl (k, l) L P pc e (TAbs t') (Atom (VClos e t') pc).
+Proof.
+  intros. destruct k; destruct l; reflexivity.
+Qed.
+  
+Lemma eval_kl_abs_inv :
+  forall k l L P pc e t' a,
+    eval_kl (k, l) L P pc e (TAbs t') a ->
+    a = Atom (VClos e t') pc.
+Proof.
+  introv Heval.
+  destruct a as [v1 l1]; destruct v1 as [b1 | n1 | e1 t1];
+  destruct k; destruct l; inversion Heval; auto.
+Qed.
 
 Definition eval (L : two) (P : value -> value -> Prop)
            (pc : two) (e : env) (t : term) (a : atom) : Prop :=
