coq/two/LambdaTwoNI.v
@@ -4,116 +4,64 @@ Require Import LibTactics.
 
 Section NI.
 
-Lemma non_interference_n :
+Lemma eval_kl_subset_n :
   forall n,
-    forall k k' L P pc e e' t a a',
-      k + k' < n ->
-      env_LPequiv L P e e' ->
-      eval_k k L P pc e t a ->
-      eval_k k' L P pc e' t a' ->
-      (forall v, P v v) ->
-      atom_LPequiv L P a a'.
+    forall k l,
+      k + l < n ->
+      (forall L P pc e t a,
+         eval_kl (k, l) L P pc e t a ->
+         eval_kl (S k, l) L P pc e t a) /\
+      (forall L P pc e t a,
+         eval_kl (k, S l) L P pc e t a ->
+         eval_kl (k, l) L P pc e t a).
 Proof.
-  intro n. induction n; introv Hn He Heval1 Heval2 Prefl.
-  - inversion Hn.
+  intro n. induction n; auto. split; introv Heval.
+  - destruct t.
+    + (* TBool *) 
+      apply eval_kl_bool_inv in Heval.
+      subst. apply eval_kl_bool.
+    + (* TNat *)
+      apply eval_kl_nat_inv in Heval. subst.
+      apply eval_kl_nat.
+    + (* TVar *)
+      apply eval_kl_var_inv in Heval. destruct Heval as [v' [l' [H1 H2]]].
+      subst. apply eval_kl_var. assumption.
+    + (* TAbs *)
+      apply eval_kl_abs_inv in Heval.
+      subst. apply eval_kl_abs.
+    + (* TApp *)
+      admit.
+    + (* TDecl *)
+      admit.
   - destruct t.
     + (* TBool *)
-      destruct k; destruct k'; 
-      (inversion Heval1; inversion Heval2;
-       destruct L; destruct pc; [
-         right; left; auto |
-         left; auto |
-         right; right; auto |
-         right; right; auto
-      ]).
+      apply eval_kl_bool_inv in Heval.
+      subst. apply eval_kl_bool.
     + (* TNat *)
-      destruct k; destruct k'; 
-      (inversion Heval1; inversion Heval2;
-       destruct L; destruct pc; [
-         right; left; auto |
-         left; auto |
-         right; right; auto |
-         right; right; auto
-      ]).
+      apply eval_kl_nat_inv in Heval.
+      subst. apply eval_kl_nat.
     + (* TVar *)
-      destruct k; destruct k';
-      inversion Heval1 as [v1 Ha1]; destruct Ha1 as [l1 [Ha1 Ha]];
-      inversion Heval2 as [v2 Ha2]; destruct Ha2 as [l2 [Ha2 Ha']]; subst;
-      assert (Ha1a2: atom_LPequiv L P (Atom v1 l1) (Atom v2 l2)) by
-          (eapply list_forall2_atIndex; eauto);
-      assert (l2 = l1) by (apply atom_LPequiv_lab_inv in Ha1a2; auto); subst;
-      destruct pc; destruct l1; simpl; auto;
-      apply atom_LPequiv_raise; auto.
+      apply eval_kl_var_inv in Heval. destruct Heval as [v' [l' [H1 H2]]].
+      subst. apply eval_kl_var. assumption.
     + (* TAbs *)
-      destruct k; destruct k'; 
-      (inversion Heval1; inversion Heval2;
-       destruct L; destruct pc; [
-         right; left; auto |
-         left; auto |
-         right; right; auto |
-         right; right; auto
-      ]).
+      apply eval_kl_abs_inv in Heval.
+      subst. apply eval_kl_abs.
     + (* TApp *)
-      destruct k; destruct k';
-      inversion Heval1; inversion Heval2.
-      rename x into e1; rename x0 into e1'.
-      destruct H as
-          [t1' [l1 [a2 [a3 [Heval1a [Heval1b [Heval1c Ha1]]]]]]].
-      destruct H0 as
-          [t1'' [l1' [a2' [a3' [Heval2a [Heval2b [Heval2c Ha2]]]]]]].
-      subst.
-      remember (Atom (VClos e1 t1') l1) as a1;
-      remember (Atom (VClos e1' t1'') l1') as a1'.
-      assert (atom_LPequiv L P a1 a1') by (eapply IHn; eauto; omega); subst.
-      assert (l1' = l1) by (apply atom_LPequiv_lab_inv in H; auto); subst.
-      assert (env_LPequiv L P e1 e1' /\ t1'' = t1') by
-          (split; destruct H; destruct H; destruct_conjs; subst; auto);
-        destruct_conjs; subst.
-      assert (atom_LPequiv L P a2 a2') by
-          (apply IHn with
-           (k := k) (k' := k') (pc := pc) (e := e) (e' := e') (t := t2);
-           try omega; auto).
-      assert (env_LPequiv L P (a2 :: e1) (a2' :: e1')) by (split; auto).
-      eapply IHn; eauto; omega.
+      admit.
     + (* TDecl *)
-      destruct k; destruct k';
-      inversion Heval1; inversion Heval2.
-      rename x into e1; rename x0 into e1'.
-      destruct H as
-          [t1' [l1 [a2 [v3 [l3 [Heval1a [Heval1b [Heval1c Ha1]]]]]]]].
-      destruct H0 as
-          [t1'' [l1' [a2' [v3' [l3' [Heval2a [Heval2b [Heval2c Ha2]]]]]]]].
-      subst.
-      remember (Atom (VClos e1 t1') l1) as a1;
-      remember (Atom (VClos e1' t1'') l1') as a1'.
-      assert (atom_LPequiv L P a1 a1') by (eapply IHn; eauto; omega); subst.
-      assert (l1' = l1) by (apply atom_LPequiv_lab_inv in H; auto); subst.
-      assert (env_LPequiv L P e1 e1' /\ t1'' = t1') by
-          (split; destruct H; destruct H; destruct_conjs; subst; auto);
-        destruct_conjs; subst.
-      assert (atom_LPequiv L P a2 a2') by
-          (apply IHn with
-           (k := k) (k' := k') (pc := pc) (e := e) (e' := e') (t := t2);
-           try omega; auto).
-      assert (env_LPequiv L P (a2 :: e1) (a2' :: e1')) by (split; auto).
-      assert (atom_LPequiv L P (Atom v3 l3) (Atom v3' l3')) by
-          (eapply IHn; eauto; omega).
-      assert (l3' = l3) by (apply atom_LPequiv_lab_inv in H3; auto); subst.
-      destruct l3; destruct_conjs; subst; auto.
-      assert (value_LPequiv L P v3 v3').
-      eapply H6; eauto.
-      Admitted.
+      admit.
+Qed.
 
-Theorem non_interference :
-  forall k k' L P pc e e' t a a',
-    env_LPequiv L P e e' ->
-    eval_k k L P pc e t a ->
-    eval_k k' L P pc e' t a' ->
-    (forall v, P v v) ->
-    atom_LPequiv L P a a'.
+Lemma eval_kl_subset :
+  forall k l,
+    (forall L P pc e t a,
+       eval_kl (k, l) L P pc e t a ->
+       eval_kl (S k, l) L P pc e t a) /\
+    (forall L P pc e t a,
+       eval_kl (k, S l) L P pc e t a ->
+       eval_kl (k, l) L P pc e t a).
 Proof.
-  introv He Heval1 Heval2 Prefl.
-  eapply non_interference_n; eauto.
+  intros k l. apply (eval_kl_subset_n (S (k + l))). auto.
 Qed.
   
 End NI.
